theories/parabstr/scheduler.v
@@ -1,13 +1,14 @@
 From zebre Require Import
   prelude.
 From zebre.iris.bi Require Import
-  big_op.
+big_op.
 From zebre.language Require Import
   notations
   diaframe.
 From zebre.std Require Import
   opt
-  for_upto
+  array
+  domain
   spmc_future.
 From zebre.parabstr Require Export
   base.
@@ -16,13 +17,23 @@ From zebre.parabstr Require Import
 From zebre Require Import
   options.
 
-Implicit Types v t task : val.
+Implicit Types not_killed : bool.
+Implicit Types v t hub task : val.
 
 #[local] Notation "'hub'" := (
+  in_type "t" 0
+)(in custom zebre_proj
+).
+#[local] Notation "'domains'" := (
+  in_type "t" 1
+)(in custom zebre_proj
+).
+
+#[local] Notation "'context_hub'" := (
   in_type "context" 0
 )(in custom zebre_proj
 ).
-#[local] Notation "'id'" := (
+#[local] Notation "'context_id'" := (
   in_type "context" 1
 )(in custom zebre_proj
 ).
@@ -40,30 +51,37 @@ Section ws_deques.
     λ: "ctx" "task",
       "task" "ctx".
 
-  #[local] Definition scheduler_worker_aux : val :=
+  #[local] Definition scheduler_step : val :=
     λ: "ctx",
-      let: "task" := ws_hub_pop_steal ws_hub "ctx".<hub> "ctx".<id> scheduler_max_round in
-      scheduler_execute "ctx" "task".
+      match: ws_hub_pop_steal ws_hub "ctx".<context_hub> "ctx".<context_id> scheduler_max_round with
+      | Some "task" =>
+          scheduler_execute "ctx" "task" ;;
+          #true
+      | None =>
+          #false
+      end.
+
   #[local] Definition scheduler_worker : val :=
     rec: "scheduler_worker" "ctx" :=
-      scheduler_worker_aux "ctx" ;;
-      "scheduler_worker" "ctx".
+      if: scheduler_step "ctx" then
+        "scheduler_worker" "ctx".
 
   Definition scheduler_create : val :=
     λ: "sz",
-      let: "t" := ws_hub.(ws_hub_create) (#1 + "sz") in
-      for: "i" := #1 to #1 + "sz" begin
-        Fork (scheduler_worker ("t", "i"))
-      end ;;
-      ("t", #0).
+      let: "hub" := ws_hub.(ws_hub_create) (#1 + "sz") in
+      let: "doms" := array_initi "sz" (λ: "i",
+        domain_spawn (λ: <>, scheduler_worker ("hub", #1 + "i"))
+      ) in
+      ("hub", "doms").
 
   #[using="ws_hub"]
-  Definition scheduler_run :=
-    scheduler_execute.
+  Definition scheduler_run : val :=
+    λ: "t" "task",
+      scheduler_execute ("t".<hub>, #0) "task".
 
   Definition scheduler_silent_async : val :=
     λ: "ctx" "task",
-      ws_hub.(ws_hub_push) "ctx".<hub> "ctx".<id> "task".
+      ws_hub.(ws_hub_push) "ctx".<context_hub> "ctx".<context_id> "task".
 
   Definition scheduler_async : val :=
     λ: "ctx" "task",
@@ -79,16 +97,23 @@ Section ws_deques.
       | Some "res" =>
           "res"
       | None =>
-          scheduler_worker_aux "ctx" ;;
+          scheduler_step "ctx" ;;
           "scheduler_await" "ctx" "fut"
       end.
+
+  Definition scheduler_kill : val :=
+    λ: "t",
+      ws_hub.(ws_hub_kill) "t".<hub> ;;
+      array_iter "t".<domains> domain_join.
 End ws_deques.
 
 Class SchedulerG Σ `{zebre_G : !ZebreG Σ} := {
+  #[local] scheduler_G_domain_G :: DomainG Σ ;
   #[local] scheduler_G_future_G :: SpmcFutureG Σ ;
 }.
 
 Definition scheduler_Σ := #[
+  domain_Σ ;
   spmc_future_Σ
 ].
 #[global] Instance subG_scheduler_Σ Σ `{zebre_G : !ZebreG Σ} :
@@ -102,25 +127,39 @@ Section scheduler_G.
   Context `{scheduler_G : SchedulerG Σ}.
   Context (ws_hub : ws_hub Σ).
 
-  #[local] Definition scheduler_task t task : iProp Σ :=
+  #[local] Definition scheduler_task hub task Ψ : iProp Σ :=
     ∀ i,
-    ws_hub.(ws_hub_owner) t i -∗
-    WP task (t, #i)%V {{ _,
-      ws_hub.(ws_hub_owner) t i
+    ws_hub.(ws_hub_owner) hub i -∗
+    WP task (hub, #i)%V {{ v,
+      ws_hub.(ws_hub_owner) hub i ∗
+      Ψ v
     }}.
-  #[local] Definition scheduler_inv_inner t : iProp Σ :=
+  #[local] Definition scheduler_inv_inner hub : iProp Σ :=
     ∃ tasks,
-    ws_hub.(ws_hub_model) t tasks ∗
+    ws_hub.(ws_hub_model) hub tasks ∗
     [∗ mset] task ∈ tasks,
-      scheduler_task t task.
-  Definition scheduler_inv t : iProp Σ :=
-    ws_hub.(ws_hub_inv) t (nroot.@"hub") ∗
-    inv (nroot.@"inv") (scheduler_inv_inner t).
+      scheduler_task hub task (λ _, True).
+  #[local] Definition scheduler_inv hub : iProp Σ :=
+    ws_hub.(ws_hub_inv) hub (nroot.@"hub") ∗
+    inv (nroot.@"inv") (scheduler_inv_inner hub).
 
-  Definition scheduler_context t ctx : iProp Σ :=
-    ∃ (i : nat),
-    ⌜ctx = (t, #i)%V⌝ ∗
-    ws_hub.(ws_hub_owner) t i.
+  Definition scheduler_model t : iProp Σ :=
+    ∃ hub v_doms doms,
+    ⌜t = (hub, v_doms)%V⌝ ∗
+    scheduler_inv hub ∗
+    ws_hub.(ws_hub_owner) hub 0 ∗
+    array_model v_doms DfracDiscarded doms ∗
+    [∗ list] dom ∈ doms,
+      domain_model dom (λ res, ⌜res = ()%V⌝).
+
+  #[local] Definition scheduler_context' ctx (i : nat) : iProp Σ :=
+    ∃ hub,
+    ⌜ctx = (hub, #i)%V⌝ ∗
+    scheduler_inv hub ∗
+    ws_hub.(ws_hub_owner) hub i.
+  Definition scheduler_context ctx : iProp Σ :=
+    ∃ i,
+    scheduler_context' ctx i.
 
   #[using="ws_hub"]
   Definition scheduler_future :=
@@ -132,178 +171,184 @@ Section scheduler_G.
     solve_proper.
   Qed.
 
-  #[global] Instance scheduler_inv_persistent t :
-    Persistent (scheduler_inv t).
-  Proof.
-    apply _.
-  Qed.
   #[global] Instance scheduler_future_persistent fut Ψ :
     Persistent (scheduler_future fut Ψ).
   Proof.
     apply _.
   Qed.
 
-  #[local] Lemma scheduler_execute_spec t i task :
-    (0 ≤ i)%Z →
+  #[local] Lemma scheduler_execute_spec hub i task Ψ :
     {{{
-      ws_hub.(ws_hub_owner) t (Z.to_nat i) ∗
-      scheduler_task t task
+      ws_hub.(ws_hub_owner) hub i ∗
+      scheduler_task hub task Ψ
     }}}
-      scheduler_execute (t, #i)%V task
-    {{{ res,
-      RET res;
-      ws_hub.(ws_hub_owner) t (Z.to_nat i)
-    }}}.
-  Proof.
-    iIntros "%Hi %Φ (Hhub_owner & Htask) HΦ".
-
-    iSpecialize ("Htask" with "Hhub_owner").
-    rewrite Z2Nat.id //. iSteps.
-  Qed.
-
-  #[local] Lemma scheduler_worker_aux_spec t i :
-    (0 ≤ i)%Z →
-    {{{
-      scheduler_inv t ∗
-      ws_hub.(ws_hub_owner) t (Z.to_nat i)
-    }}}
-      scheduler_worker_aux ws_hub (t, #i)%V
-    {{{ res,
-      RET res;
-      ws_hub.(ws_hub_owner) t (Z.to_nat i)
-    }}}.
-  Proof.
-    iIntros "%Hi %Φ ((#Hhub_inv & #Hinv) & Hhub_owner) HΦ".
-
-    wp_rec.
-
-    awp_smart_apply (ws_hub_pop_steal_spec with "[$Hhub_inv $Hhub_owner]") without "HΦ"; [lia.. |].
-    iInv "Hinv" as "(%tasks & >Hhub_model & Htasks)".
-    iAaccIntro with "Hhub_model"; first iSteps. iIntros "%task %tasks' (-> & Hhub_model)".
-    iDestruct (big_sepMS_disj_union with "Htasks") as "(Htask & Htasks)".
-    rewrite big_sepMS_singleton.
-    iSplitR "Htask"; first iSteps.
-    iIntros "!> Hhub_owner HΦ".
-
-    wp_smart_apply (scheduler_execute_spec with "[$Hhub_owner $Htask] HΦ"); first done.
-  Qed.
-  #[local] Lemma scheduler_worker_spec t i :
-    (0 ≤ i)%Z →
-    {{{
-      scheduler_inv t ∗
-      ws_hub.(ws_hub_owner) t (Z.to_nat i)
-    }}}
-      scheduler_worker ws_hub (t, #i)%V
-    {{{
-      RET (); True
-    }}}.
-  Proof.
-    iIntros "%Hi %Φ (#Hinv & Hhub_owner) HΦ".
-
-    iLöb as "HLöb".
-
-    wp_rec.
-    wp_apply (scheduler_worker_aux_spec with "[$Hinv $Hhub_owner]") as (res) "Hhub_owner"; first done.
-    wp_smart_apply ("HLöb" with "Hhub_owner HΦ").
-  Qed.
-
-  Lemma scheduler_create_spec sz :
-    (0 ≤ sz)%Z →
-    {{{ True }}}
-      scheduler_create ws_hub #sz
-    {{{ t ctx,
-      RET ctx;
-      scheduler_inv t ∗
-      scheduler_context t ctx
-    }}}.
-  Proof.
-    iIntros "%Hsz %Φ _ HΦ".
-
-    wp_rec.
-    wp_smart_apply (ws_hub_create_spec with "[//]") as (t) "(#Hhub_inv & Hhub_model & Hhub_owners)"; first lia.
-
-    iMod (inv_alloc _ _ (scheduler_inv_inner t) with "[Hhub_model]") as "#Hinv".
-    { iSteps. rewrite big_sepMS_empty //. }
-
-    rewrite Z.add_1_l Z2Nat.inj_succ // -cons_seq.
-    iDestruct "Hhub_owners" as "(Hhub_owner & Hhub_owners)".
-    wp_smart_apply (for_upto_spec_disentangled' (λ _ _, True)%I with "[Hhub_owners]"); last first.
-    { iSteps. iExists 0. iSteps. }
-    iApply (big_sepL_mono_strong with "Hhub_owners").
-    { rewrite !seq_length. lia. }
-    iIntros "!>" (δ i1 i2 ((-> & Hi1)%lookup_seq & (-> & Hi2)%lookup_seq)) "Hhub_owner %i -> /=".
-    wp_smart_apply (wp_fork with "[Hhub_owner]"); last iSteps. iModIntro.
-    rewrite Z.add_1_l -Nat2Z.inj_succ.
-    wp_smart_apply (scheduler_worker_spec with "[$Hhub_inv $Hinv Hhub_owner]").
-    { done. }
-    { rewrite Nat2Z.id //. }
-    iSteps.
-  Qed.
-
-  Lemma scheduler_run_spec Ψ t ctx task :
-    {{{
-      scheduler_inv t ∗
-      scheduler_context t ctx ∗
-      ( ∀ ctx,
-        scheduler_context t ctx -∗
-        WP task ctx {{ v,
-          scheduler_context t ctx ∗
-          Ψ v
-        }}
-      )
-    }}}
-      scheduler_run ws_hub ctx task
+      scheduler_execute (hub, #i)%V task
     {{{ v,
       RET v;
-      scheduler_context t ctx ∗
+      ws_hub.(ws_hub_owner) hub i ∗
       Ψ v
     }}}.
   Proof.
     iSteps.
   Qed.
 
-  Lemma scheduler_silent_async_spec t ctx task :
+  #[local] Lemma scheduler_step_spec ctx :
     {{{
-      scheduler_inv t ∗
-      scheduler_context t ctx ∗
+      scheduler_context ctx
+    }}}
+      scheduler_step ws_hub ctx
+    {{{ not_killed,
+      RET #not_killed;
+      scheduler_context ctx
+    }}}.
+  Proof.
+    iIntros "%Φ (%i & %hub & -> & (#Hhub_inv & #Hinv) & Hhub_owner) HΦ".
+
+    wp_rec.
+
+    awp_smart_apply (ws_hub_pop_steal_spec with "[$Hhub_inv $Hhub_owner]") without "HΦ"; [done | lia.. |].
+    iInv "Hinv" as "(%tasks & >Hhub_model & Htasks)".
+    iAaccIntro with "Hhub_model"; first iSteps.
+    iIntros ([task |]) "Hhub_model !>"; last first.
+
+    - iSplitL; first iSteps.
+      iIntros "Hhub_owner HΦ". clear.
+
+      wp_pures.
+      iApply "HΦ".
+      iExists i. iSteps.
+
+    - iDestruct "Hhub_model" as "(%tasks' & -> & Hhub_model)".
+      iDestruct (big_sepMS_disj_union with "Htasks") as "(Htask & Htasks)".
+      rewrite big_sepMS_singleton.
+      iSplitR "Htask"; first iSteps.
+      iIntros "Hhub_owner HΦ". clear- scheduler_G.
+
+      wp_smart_apply (scheduler_execute_spec with "[$Hhub_owner $Htask]") as (res) "(Hhub_owner & _)".
+      wp_pures.
+      iApply "HΦ".
+      iExists i. iSteps.
+  Qed.
+
+  #[local] Lemma scheduler_worker_spec ctx :
+    {{{
+      scheduler_context ctx
+    }}}
+      scheduler_worker ws_hub ctx
+    {{{
+      RET (); True
+    }}}.
+  Proof.
+    iIntros "%Φ Hctx HΦ".
+
+    iLöb as "HLöb".
+
+    wp_rec.
+    wp_apply (scheduler_step_spec with "Hctx") as ([]) "Hctx"; last iSteps.
+    wp_smart_apply ("HLöb" with "Hctx HΦ").
+  Qed.
+
+  Lemma scheduler_create_spec sz :
+    (0 ≤ sz)%Z →
+    {{{ True }}}
+      scheduler_create ws_hub #sz
+    {{{ t,
+      RET t;
+      scheduler_model t
+    }}}.
+  Proof.
+    iIntros "%Hsz %Φ _ HΦ".
+
+    wp_rec.
+    wp_smart_apply (ws_hub_create_spec with "[//]") as (t) "(#Hhub_inv & Hhub_model & Hhub_owners)"; first lia.
+    rewrite Z2Nat.inj_add //.
+    iDestruct "Hhub_owners" as "(Hhub_owner & Hhub_owners)".
+
+    iMod (inv_alloc _ _ (scheduler_inv_inner t) with "[Hhub_model]") as "#Hinv".
+    { iSteps. rewrite big_sepMS_empty //. }
+
+    pose Ψ res : iProp Σ := (
+      ⌜res = ()%V⌝
+    )%I.
+    wp_smart_apply (array_initi_spec_disentangled' (λ _ dom, domain_model dom Ψ) with "[Hhub_owners]") as (v_doms doms) "(_ & Hv_doms & Hdoms)"; first done.
+    { iApply (big_sepL_mono_strong with "Hhub_owners").
+      { rewrite !seq_length. lia. }
+      iIntros "!>" (k i1 i2 ((-> & Hi1)%lookup_seq & (-> & Hi2)%lookup_seq)) "Hhub_owner".
+      wp_smart_apply (domain_spawn_spec Ψ with "[Hhub_owner]"); last iSteps.
+      wp_smart_apply (scheduler_worker_spec with "[Hhub_owner]"); last iSteps.
+      rewrite Z.add_1_l -Nat2Z.inj_succ. iExists _. iSteps.
+    }
+    iMod (array_model_persist with "Hv_doms") as "#Hv_doms".
+    iSteps.
+  Qed.
+
+  Lemma scheduler_run_spec Ψ t task :
+    {{{
+      scheduler_model t ∗
       ( ∀ ctx,
-        scheduler_context t ctx -∗
+        scheduler_context ctx -∗
+        WP task ctx {{ v,
+          scheduler_context ctx ∗
+          Ψ v
+        }}
+      )
+    }}}
+      scheduler_run ws_hub t task
+    {{{ v,
+      RET v;
+      scheduler_model t ∗
+      Ψ v
+    }}}.
+  Proof.
+    iIntros "%Φ ((%hub & %v_doms & %doms & -> & (#Hhub_inv & #Hinv) & Hhub_owner & Hv_doms & Hdoms) & Htask) HΦ".
+
+    wp_rec.
+    wp_smart_apply (scheduler_execute_spec _ 0 _ Ψ with "[$Hhub_owner Htask]") as (v) "(Hhub_owner & HΨ)"; last iSteps. iIntros "%i Hhub_owner".
+    wp_apply (wp_wand with "(Htask [Hhub_owner])"); last iSteps.
+    iExists i. iSteps.
+  Qed.
+
+  Lemma scheduler_silent_async_spec ctx task :
+    {{{
+      scheduler_context ctx ∗
+      ( ∀ ctx,
+        scheduler_context ctx -∗
         WP task ctx {{ res,
-          scheduler_context t ctx
+          scheduler_context ctx
         }}
       )
     }}}
       scheduler_silent_async ws_hub ctx task
     {{{
       RET ();
-      scheduler_context t ctx
+      scheduler_context ctx
     }}}.
   Proof.
-    iIntros "%Φ ((#Hhub_inv & #Hinv) & (%i & -> & Hhub_owner) & Htask) HΦ".
+    iIntros "%Φ ((%i & %hub & -> & (#Hhub_inv & #Hinv) & Hhub_owner) & Htask) HΦ".
 
     wp_rec.
 
-    awp_smart_apply (ws_hub_push_spec with "[$Hhub_inv Hhub_owner]") without "HΦ".
-    { lia. }
-    { rewrite Nat2Z.id //. }
+    awp_smart_apply (ws_hub_push_spec with "[$Hhub_inv $Hhub_owner]") without "HΦ"; first done.
     iInv "Hinv" as "(%tasks & >Hhub_model & Htasks)".
     iAaccIntro with "Hhub_model". { iFrame. iSteps. } iIntros "Hhub_model".
     iSplitL.
     { iExists _. iFrame. rewrite big_sepMS_singleton. iIntros "!> !> %j Hhub_owner".
-      wp_smart_apply (wp_wand with "(Htask [Hhub_owner])") as (res) "(%_j & %Heq & Hhub_owner)"; first iSteps.
-      injection Heq as [= <-%(inj _)]. iSteps.
+      wp_smart_apply (wp_wand with "(Htask [Hhub_owner])"); last iSteps.
+      iExists j. iSteps.
     }
-    rewrite Nat2Z.id. iSteps.
+    iIntros "!> Hhub_owner HΦ". clear.
+
+    iApply "HΦ".
+    iExists i. iSteps.
   Qed.
 
-  Lemma scheduler_async_spec Ψ t ctx task :
+  Lemma scheduler_async_spec Ψ ctx task :
     {{{
-      scheduler_inv t ∗
-      scheduler_context t ctx ∗
+      scheduler_context ctx ∗
       ( ∀ ctx,
-        scheduler_context t ctx -∗
+        scheduler_context ctx -∗
         WP task ctx {{ v,
-          scheduler_context t ctx ∗
+          scheduler_context ctx ∗
           □ Ψ v
         }}
       )
@@ -311,45 +356,66 @@ Section scheduler_G.
       scheduler_async ws_hub ctx task
     {{{ fut,
       RET fut;
-      scheduler_context t ctx ∗
+      scheduler_context ctx ∗
       scheduler_future fut Ψ
     }}}.
   Proof.
-    iIntros "%Φ (#Hinv & Hctx & Htask) HΦ".
+    iIntros "%Φ (Hctx & Htask) HΦ".
 
     wp_rec.
     wp_smart_apply (spmc_future_create_spec with "[//]") as (fut) "(#Hfut_inv & Hfut_producer)".
-    wp_smart_apply (scheduler_silent_async_spec with "[$Hinv $Hctx Htask Hfut_producer]"); last iSteps.
-    clear ctx. iIntros "%ctx Hctx".
-    wp_smart_apply (wp_wand with "(Htask Hctx)") as (v) "(Hctx & HΨ)".
-    wp_apply (spmc_future_set_spec with "[$Hfut_inv $Hfut_producer $HΨ]") as "_".
-    iFrame.
+    wp_smart_apply (scheduler_silent_async_spec with "[$Hctx Htask Hfut_producer]") as "Hctx".
+    { clear ctx. iIntros "%ctx Hctx".
+      wp_smart_apply (wp_wand with "(Htask Hctx)") as (v) "(Hctx & HΨ)".
+      wp_apply (spmc_future_set_spec with "[$Hfut_inv $Hfut_producer $HΨ]") as "_ //".
+    }
+    wp_pures.
+    iApply ("HΦ" with "[$Hctx $Hfut_inv]").
   Qed.
 
-  Lemma scheduler_await_spec t ctx fut Ψ :
+  Lemma scheduler_await_spec ctx fut Ψ :
     {{{
-      scheduler_inv t ∗
-      scheduler_context t ctx ∗
+      scheduler_context ctx ∗
       scheduler_future fut Ψ
     }}}
       scheduler_await ws_hub ctx fut
     {{{ v,
       RET v;
-      scheduler_context t ctx ∗
+      scheduler_context ctx ∗
       Ψ v
     }}}.
   Proof.
-    iIntros "%Φ ((#Hhub_inv & #Hinv) & (%i & -> & Hhub_owner) & #Hfut_inv) HΦ".
+    iIntros "%Φ (Hctx & #Hfut_inv) HΦ".
 
     iLöb as "HLöb".
 
     wp_rec.
-    wp_smart_apply (spmc_future_try_get_spec with "Hfut_inv") as ([task |]) "HΨ"; first iSteps.
-    wp_smart_apply (scheduler_worker_aux_spec with "[$Hhub_inv $Hinv Hhub_owner]") as (res) "Hhub_owner".
-    { lia. }
-    { rewrite Nat2Z.id //. }
-    rewrite Nat2Z.id.
-    wp_smart_apply ("HLöb" with "Hhub_owner HΦ").
+    wp_smart_apply (spmc_future_try_get_spec with "Hfut_inv") as ([task |]) "HΨ".
+
+    - wp_pures.
+      iApply ("HΦ" with "[$Hctx $HΨ]").
+
+    - wp_smart_apply (scheduler_step_spec with "Hctx") as (not_killed) "Hctx".
+      wp_smart_apply ("HLöb" with "Hctx HΦ").
+  Qed.
+
+  Lemma scheduler_kill_spec t :
+    {{{
+      scheduler_model t
+    }}}
+      scheduler_kill ws_hub t
+    {{{
+      RET (); True
+    }}}.
+  Proof.
+    iIntros "%Φ (%hub & %v_doms & %doms & -> & (#Hhub_inv & #Hinv) & Hhub_owner & Hv_doms & Hdoms) HΦ".
+
+    wp_rec.
+    wp_smart_apply (ws_hub_kill_spec with "Hhub_inv") as "_".
+    wp_smart_apply (array_iter_spec_disentangled' (λ _ _, True)%I with "[$Hv_doms Hdoms]"); last iSteps.
+    iApply (big_sepL_impl with "Hdoms"). iIntros "!> %i %dom _ Hdom".
+    wp_apply (domain_join_spec with "Hdom").
+    iSteps.
   Qed.
 End scheduler_G.
 
@@ -358,7 +424,8 @@ End scheduler_G.
 #[global] Opaque scheduler_silent_async.
 #[global] Opaque scheduler_async.
 #[global] Opaque scheduler_await.
+#[global] Opaque scheduler_kill.
 
-#[global] Opaque scheduler_inv.
+#[global] Opaque scheduler_model.
 #[global] Opaque scheduler_context.
 #[global] Opaque scheduler_future.
