theories/parabstr/ws_hub.v
@@ -10,6 +10,7 @@ From zebre.parabstr Require Export
 From zebre Require Import
   options.
 
+Implicit Types killed : bool.
 Implicit Types v t : val.
 
 Record ws_hub `{zebre_G : !ZebreG Σ} := {
@@ -19,6 +20,8 @@ Record ws_hub `{zebre_G : !ZebreG Σ} := {
   ws_hub_pop : val ;
   ws_hub_try_steal : val ;
   ws_hub_steal : val ;
+  ws_hub_killed : val ;
+  ws_hub_kill : val ;
 
   ws_hub_inv : val → namespace → iProp Σ ;
   ws_hub_model : val → gmultiset val → iProp Σ ;
@@ -46,11 +49,11 @@ Record ws_hub `{zebre_G : !ZebreG Σ} := {
         ws_hub_owner t i
     }}} ;
 
-  ws_hub_push_spec t ι i v :
-    (0 ≤ i)%Z →
+  ws_hub_push_spec t ι i i_ v :
+    i = Z.of_nat i_ →
     <<<
       ws_hub_inv t ι ∗
-      ws_hub_owner t (Z.to_nat i)
+      ws_hub_owner t i_
     | ∀∀ vs,
       ws_hub_model t vs
     >>>
@@ -58,7 +61,7 @@ Record ws_hub `{zebre_G : !ZebreG Σ} := {
     <<<
       ws_hub_model t ({[+v+]} ⊎ vs)
     | RET ();
-      ws_hub_owner t (Z.to_nat i)
+      ws_hub_owner t i_
     >>> ;
 
   ws_hub_push_foreign_spec t ι v :
@@ -73,11 +76,11 @@ Record ws_hub `{zebre_G : !ZebreG Σ} := {
     | RET (); True
     >>> ;
 
-  ws_hub_pop_spec t ι i :
-    (0 ≤ i)%Z →
+  ws_hub_pop_spec t ι i i_ :
+    i = Z.of_nat i_ →
     <<<
       ws_hub_inv t ι ∗
-      ws_hub_owner t (Z.to_nat i)
+      ws_hub_owner t i_
     | ∀∀ vs,
       ws_hub_model t vs
     >>>
@@ -93,16 +96,16 @@ Record ws_hub `{zebre_G : !ZebreG Σ} := {
           ws_hub_model t vs'
       end
     | RET o;
-      ws_hub_owner t (Z.to_nat i)
+      ws_hub_owner t i_
     >>> ;
 
-  ws_hub_try_steal_spec t ι i max_round_noyield max_round_yield :
-    (0 ≤ i)%Z →
+  ws_hub_try_steal_spec t ι i i_ max_round_noyield max_round_yield :
+    i = Z.of_nat i_ →
     (0 ≤ max_round_noyield)%Z →
     (0 ≤ max_round_yield)%Z →
     <<<
       ws_hub_inv t ι ∗
-      ws_hub_owner t (Z.to_nat i)
+      ws_hub_owner t i_
     | ∀∀ vs,
       ws_hub_model t vs
     >>>
@@ -118,36 +121,62 @@ Record ws_hub `{zebre_G : !ZebreG Σ} := {
           ws_hub_model t vs'
       end
     | RET o;
-      ws_hub_owner t (Z.to_nat i)
+      ws_hub_owner t i_
     >>> ;
 
-  ws_hub_steal_spec t ι i max_round_noyield max_round_yield :
-    (0 ≤ i)%Z →
+  ws_hub_steal_spec t ι i i_ max_round_noyield max_round_yield :
+    i = Z.of_nat i_ →
     (0 ≤ max_round_noyield)%Z →
     (0 ≤ max_round_yield)%Z →
     <<<
       ws_hub_inv t ι ∗
-      ws_hub_owner t (Z.to_nat i)
+      ws_hub_owner t i_
     | ∀∀ vs,
       ws_hub_model t vs
     >>>
       ws_hub_steal t #i (#max_round_noyield, #max_round_yield)%V @ ↑ι
     <<<
-      ∃∃ v vs',
-      ⌜vs = {[+v+]} ⊎ vs'⌝ ∗
-      ws_hub_model t vs'
-    | RET v;
-      ws_hub_owner t (Z.to_nat i)
+      ∃∃ o,
+      match o with
+      | None =>
+          ws_hub_model t vs
+      | Some v =>
+          ∃ vs',
+          ⌜vs = {[+v+]} ⊎ vs'⌝ ∗
+          ws_hub_model t vs'
+      end
+    | RET o;
+      ws_hub_owner t i_
     >>> ;
+
+  ws_hub_killed_spec t ι :
+    {{{
+      ws_hub_inv t ι
+    }}}
+      ws_hub_killed t
+    {{{ killed,
+      RET #killed; True
+    }}} ;
+
+  ws_hub_kill_spec t ι:
+    {{{
+      ws_hub_inv t ι
+    }}}
+      ws_hub_kill t
+    {{{
+      RET (); True
+    }}} ;
 }.
 #[global] Arguments ws_hub _ {_} : assert.
-#[global] Arguments Build_ws_hub {_ _ _ _ _ _ _ _ _ _ _ _ _} _ _ _ _ _ _ _ : assert.
+#[global] Arguments Build_ws_hub {_ _ _ _ _ _ _ _ _ _ _ _ _ _ _} _ _ _ _ _ _ _ _ _ : assert.
 #[global] Opaque ws_hub_create.
 #[global] Opaque ws_hub_push.
 #[global] Opaque ws_hub_push_foreign.
 #[global] Opaque ws_hub_pop.
 #[global] Opaque ws_hub_try_steal.
 #[global] Opaque ws_hub_steal.
+#[global] Opaque ws_hub_killed.
+#[global] Opaque ws_hub_kill.
 
 Section zebre_G.
   Context `{zebre_G : !ZebreG Σ}.
@@ -165,19 +194,19 @@ Section zebre_G.
   Definition ws_hub_pop_steal : val :=
     λ: "t" "i" "max_round",
       match: ws_hub.(ws_hub_pop) "t" "i" with
-      | Some "v" =>
-          "v"
+      | Some <> as "res" =>
+          "res"
       | None =>
           ws_hub.(ws_hub_steal) "t" "i" "max_round"
       end.
 
-  Lemma ws_hub_pop_try_steal_spec t ι i max_round_noyield max_round_yield :
-    (0 ≤ i)%Z →
+  Lemma ws_hub_pop_try_steal_spec t ι i i_ max_round_noyield max_round_yield :
+    i = Z.of_nat i_ →
     (0 ≤ max_round_noyield)%Z →
     (0 ≤ max_round_yield)%Z →
     <<<
       ws_hub.(ws_hub_inv) t ι ∗
-      ws_hub.(ws_hub_owner) t (Z.to_nat i)
+      ws_hub.(ws_hub_owner) t i_
     | ∀∀ vs,
       ws_hub.(ws_hub_model) t vs
     >>>
@@ -193,10 +222,10 @@ Section zebre_G.
           ws_hub.(ws_hub_model) t vs'
       end
     | RET o;
-      ws_hub.(ws_hub_owner) t (Z.to_nat i)
+      ws_hub.(ws_hub_owner) t i_
     >>>.
   Proof.
-    iIntros "%Hi %Hmax_round_noyield %Hmax_round_yield !> %Φ (#Hinv & Howner) HΦ".
+    iIntros (->) "%Hmax_round_noyield %Hmax_round_yield !> %Φ (#Hinv & Howner) HΦ".
 
     wp_rec.
 
@@ -211,31 +240,37 @@ Section zebre_G.
       iSteps.
 
     - iLeft. iFrame.
-      iIntros "HΦ !> Howner". clear- Hi Hmax_round_noyield Hmax_round_yield.
+      iIntros "HΦ !> Howner". clear- Hmax_round_noyield Hmax_round_yield.
 
       wp_smart_apply (ws_hub_try_steal_spec with "[$Hinv $Howner] HΦ"); done.
   Qed.
 
-  Lemma ws_hub_pop_steal_spec t ι i max_round_noyield max_round_yield :
-    (0 ≤ i)%Z →
+  Lemma ws_hub_pop_steal_spec t ι i i_ max_round_noyield max_round_yield :
+    i = Z.of_nat i_ →
     (0 ≤ max_round_noyield)%Z →
     (0 ≤ max_round_yield)%Z →
     <<<
       ws_hub.(ws_hub_inv) t ι ∗
-      ws_hub.(ws_hub_owner) t (Z.to_nat i)
+      ws_hub.(ws_hub_owner) t i_
     | ∀∀ vs,
       ws_hub.(ws_hub_model) t vs
     >>>
       ws_hub_pop_steal t #i (#max_round_noyield, #max_round_yield)%V @ ↑ι
     <<<
-      ∃∃ v vs',
-      ⌜vs = {[+v+]} ⊎ vs'⌝ ∗
-      ws_hub.(ws_hub_model) t vs'
-    | RET v;
-      ws_hub.(ws_hub_owner) t (Z.to_nat i)
+      ∃∃ o,
+      match o with
+      | None =>
+          ws_hub_model ws_hub t vs
+      | Some v =>
+          ∃ vs',
+          ⌜vs = {[+v+]} ⊎ vs'⌝ ∗
+          ws_hub_model ws_hub t vs'
+      end
+    | RET o;
+      ws_hub_owner ws_hub t i_
     >>>.
   Proof.
-    iIntros "%Hi %Hmax_round_noyield %Hmax_round_yield !> %Φ (#Hinv & Howner) HΦ".
+    iIntros (->) "%Hmax_round_noyield %Hmax_round_yield !> %Φ (#Hinv & Howner) HΦ".
 
     wp_rec.
 
@@ -244,14 +279,14 @@ Section zebre_G.
     iAaccIntro with "Hmodel"; first iSteps. iIntros ([v |]) "Hmodel !>".
 
     - iDestruct "Hmodel" as "(%vs' & -> & Hmodel)".
-      iRight. iExists v, vs'. iFrame. iStep.
+      iRight. iExists (Some v). iStep.
       iIntros "HΦ !> Howner". clear.
 
       iSpecialize ("HΦ" with "Howner").
       iSteps.
 
     - iLeft. iFrame.
-      iIntros "HΦ !> Howner". clear- Hi Hmax_round_noyield Hmax_round_yield.
+      iIntros "HΦ !> Howner". clear- Hmax_round_noyield Hmax_round_yield.
 
       wp_smart_apply (ws_hub_steal_spec with "[$Hinv $Howner] HΦ"); done.
   Qed.
